theories/DSub/dsub_syn.v
@@ -137,9 +137,8 @@ Instance inh_tm : Inhabited tm := populate (tv inhabitant).
 Instance ids_vl : Ids vl.
 Proof. by constructor. Defined.
 
-Instance ids_tm : Ids tm := λ _, inhabitant.
-Instance ids_ty : Ids ty := λ _, inhabitant.
-Instance ids_list {A}: Ids (list A) := λ _, inhabitant.
+Instance ids_tm : Ids tm := inh_ids.
+Instance ids_ty : Ids ty := inh_ids.
 Instance ids_vls : Ids vls := _.
 Instance ids_ctx : Ids ctx := _.
 
